refine+crefine: make valid_arch_obj' stateless
Due to ARM_HYP, all architectures were conforming to an interface which
required valid_arch_obj' to depend on state. It turns out that this is
not necessary. Remove the dependency on state and clean up.

Signed-off-by: Rafal Kolanski <rafal.kolanski@proofcraft.systems>

proof/refine/Invariants_H.thy
@@ -392,7 +392,7 @@ definition valid_obj' :: "Structures_H.kernel_object \<Rightarrow> kernel_state 
   | KOUserDataDevice \<Rightarrow> True
   | KOTCB tcb \<Rightarrow> valid_tcb' tcb s
   | KOCTE cte \<Rightarrow> valid_cte' cte s
-  | KOArch ako \<Rightarrow> valid_arch_obj' ako s"
+  | KOArch ako \<Rightarrow> valid_arch_obj' ako"
 
 definition
   pspace_aligned' :: "kernel_state \<Rightarrow> bool"
