proof/refine/ARM_HYP/ArchArchAcc_R.thy
@@ -1282,8 +1282,8 @@ fun pde_vmsz_aligned' where
 
 definition
   "valid_slots' m \<equiv> case m of
-    Inl (pte, xs) \<Rightarrow> \<lambda>s. valid_pte' pte s \<and> pte_vmsz_aligned' pte
-  | Inr (pde, xs) \<Rightarrow> \<lambda>s. valid_pde' pde s \<and> pde_vmsz_aligned' pde"
+    Inl (pte, xs) \<Rightarrow> \<lambda>s. valid_pte' pte \<and> pte_vmsz_aligned' pte
+  | Inr (pde, xs) \<Rightarrow> \<lambda>s. valid_pde' pde \<and> pde_vmsz_aligned' pde"
 
 lemma createMappingEntries_valid_slots' [wp]:
   "\<lbrace>valid_objs' and
@@ -1566,7 +1566,7 @@ lemma storePDE_ctes [wp]:
 
 
 lemma storePDE_valid_objs [wp]:
-  "\<lbrace>valid_objs' and valid_pde' pde\<rbrace> storePDE p pde \<lbrace>\<lambda>_. valid_objs'\<rbrace>"
+  "\<lbrace>valid_objs' and K (valid_pde' pde) \<rbrace> storePDE p pde \<lbrace>\<lambda>_. valid_objs'\<rbrace>"
   apply (simp add: storePDE_def doMachineOp_def split_def)
   apply (rule hoare_pre)
    apply (wp hoare_drop_imps|wpc|simp)+
